theories/Labelled_Transition_System/Definitions/Convergence.v
@@ -358,9 +358,7 @@ Proof.
     destruct H4 as (a' & nb & inter).
     assert (blocking a) as not_nb.
     { eapply dual_blocks; eauto. }
-    assert (a' = co a) as eq_subst.
-    { eapply unique_nb; eauto. } subst.
-    edestruct (boomerang p (co a) a) as (p_a & Hyp).
+    edestruct (boomerang p a' a) as (p_a & Hyp).
     destruct (Hyp nb inter) as (tr_b & tr_nb).
     edestruct (nb_delay nb tr_nb l) as (p'_a & tr'_b & r' & tr'_nb & equiv').
     assert (p'_a ⇓ s1 ++ s2).
