theories/Testing_Pre_orders/May/Alternative_Preorder/Trace_Inclusion/EquivalenceTI.v
@@ -45,7 +45,7 @@ From TestingTheory Require Import ActTau gLts Bisimulation Lts_OBA Lts_OBA_FB Lt
 Theorem equivalence_ti_fw `{
   gLtsObaFWP : @gLtsObaFW P A H gLtsEqP gLtsObaP,
   gLtsObaFWQ : @gLtsObaFW Q A H gLtsEqQ gLtsObaQ,
-  gLtsT : !gLtsEq T H, gLtsObaT : !gLtsOba T, !Testing_Predicate outcome _}
+  gLtsT : !gLtsEq T H, gLtsObaT : !gLtsOba T, !Testing_Predicate outcome _} {unique_nb : UniqueDual A}
 
   {_ : Prop_of_Inter P T A dual}
   {_ : Prop_of_Inter Q T A dual}
@@ -70,7 +70,7 @@ Qed.
 Theorem equivalence_ti_fb `{
     @gLtsObaFB P A H gLtsEqP gLtsObaP, !FiniteOutputChain_LtsOba P, !FiniteImagegLts P A,
     @gLtsObaFB Q A H gLtsEqQ gLtsObaQ, !FiniteOutputChain_LtsOba Q, !FiniteImagegLts Q A,
-    @gLtsObaFB T A H gLtsEqT gLtsObaT, !FiniteOutputChain_LtsOba T, !Testing_Predicate outcome _}
+    @gLtsObaFB T A H gLtsEqT gLtsObaT, !FiniteOutputChain_LtsOba T, !Testing_Predicate outcome _} {unique_nb : UniqueDual A}
 
   {_ : Prop_of_Inter P (MO A) A fw_inter}
   {_ : Prop_of_Inter (P * MO A) T A dual}
@@ -95,7 +95,7 @@ Qed.
 Corollary may_equiv_iff_same_traces `{
   gLtsObaFWP : @gLtsObaFW P A H gLtsEqP gLtsObaP,
   gLtsObaFWQ : @gLtsObaFW Q A H gLtsEqQ gLtsObaQ,
-  gLtsT : !gLtsEq T H, gLtsObaT : !gLtsOba T, !Testing_Predicate outcome _}
+  gLtsT : !gLtsEq T H, gLtsObaT : !gLtsOba T, !Testing_Predicate outcome _} {unique_nb : UniqueDual A}
 
   {_ : Prop_of_Inter P T A dual}
   {_ : Prop_of_Inter Q T A dual}
