theories/Testing_Pre_orders/May/Alternative_Preorder/coTrace_Inclusion/SoundnessTIco.v
@@ -91,7 +91,7 @@ Proof. eapply soundness_ti_co. Qed.
 Theorem soundness_ti_co_fb `{
     @gLtsObaFB P A H gLtsEqP gLtsObaP, !FiniteOutputChain_LtsOba P, !FiniteImagegLts P A,
     @gLtsObaFB Q A H gLtsEqQ gLtsObaQ, !FiniteOutputChain_LtsOba Q, !FiniteImagegLts Q A,
-    @gLtsObaFB T A H gLtsEqT gLtsObaT, !FiniteOutputChain_LtsOba T, !Testing_Predicate outcome _}
+    @gLtsObaFB T A H gLtsEqT gLtsObaT, !FiniteOutputChain_LtsOba T, !Testing_Predicate outcome _} {unique_nb : UniqueDual A}
 
   {_ : Prop_of_Inter P (MO A) A fw_inter}
   {_ : Prop_of_Inter (P * MO A) T A dual}
