theories/Testing_Pre_orders/Must/Alternative_Preorder/Acceptance_Set/LabelAbstractionFW.v
@@ -38,7 +38,7 @@ Definition LA_prog_FW {A : Type} {H : ExtAction A} (R : relation A) : relation A
     (R μ μ' ∧ (non_blocking μ ↔ non_blocking μ') ∧ blocking (co μ) ∧ blocking (co μ')).
 
 Section LA_prog_FW.
-  Context {P A : Type} {H : ExtAction A} {gLtsP : gLts P H} {LAp : gLtsLAprog P H}
+  Context {P A : Type} {H : ExtAction A} {unique_nb : UniqueDual A} {gLtsP : gLts P H} {LAp : gLtsLAprog P H}
     `{!Prop_of_Inter P (MO A) A fw_inter}.
 
   Lemma LA_prog_FW_equivalence : Equivalence (LA_prog_FW (LA_prog P)).
