theories/Testing_Pre_orders/Must/Alternative_Preorder/Acceptance_Set/Soundness.v
@@ -1349,7 +1349,7 @@ Qed.
 
 (** ** Soundness for LTSs that can be lifted to forwarders *)
 Lemma soundness 
-  `{@gLtsObaFB P A H gLtsEqP gLtsObaP, !FiniteOutputChain_LtsOba P, !FiniteImagegLts P A}
+  `{@gLtsObaFB P A H gLtsEqP gLtsObaP, !FiniteOutputChain_LtsOba P, !FiniteImagegLts P A} {unique_nb : UniqueDual A}
   `{@gLtsObaFB Q A H gLtsEqQ gLtsObaQ, !FiniteOutputChain_LtsOba Q, !FiniteImagegLts Q A}
   `{@gLtsObaFB T A H gLtsEqT gLtsObaT, !FiniteOutputChain_LtsOba T, !CountablegLts T A}
 
