theories/Testing_Pre_orders/Must/Alternative_Preorder/Co_Inductive_Acceptance_Set/Equivalence/EquivalenceCI.v
@@ -58,6 +58,7 @@ Section eq_contextual.
   Context `{P : Type}.
   Context `{Q : Type}.
   Context `{H : !ExtAction A}.
+  Context {unique_nb : UniqueDual A}.
 
   Context `{@gLtsOba P A H gLtsEqP, !FiniteImagegLts P A}.
   Context `{@gLtsOba Q A H gLtsEqQ, !FiniteImagegLts Q A}.
