theories/Testing_Pre_orders/Must/Alternative_Preorder/Failure_Set/EquivalenceFMS.v
@@ -124,6 +124,7 @@ Section failure_set_preorder.
   Context `{P : Type}.
   Context `{Q : Type}.
   Context `{H : !ExtAction A}.
+  Context {unique_nb : UniqueDual A}.
 
   Context `{@gLtsOba P A H gLtsEqP, !FiniteImagegLts P A}.
   Context `{@gLtsOba Q A H gLtsEqQ, !FiniteImagegLts Q A}.
